Use a slightly redundant def for isChain (makes proofa easier).

src/dafny/beacon/forkchoice/ForkChoiceTypes.dfy
@@ -106,6 +106,27 @@ module ForkChoiceTypes {
     {
         |xr| >= 1
         &&
+        (forall i :: 0 <= i < |xr| ==> xr[i] in store.blocks.Keys)
+        // xr[0] in store.blocks.Keys
+        &&  
+        store.blocks[xr[|xr| - 1]].slot == 0 
+        && 
+        if |xr| == 1 then 
+            //  last block with slot 0 is assumed to be a chain.
+            // true
+            store.blocks[xr[0]].slot == 0 
+        else 
+            // xr[1] in store.blocks.Keys
+            && store.blocks[xr[0]].parent_root == xr[1] 
+            && store.blocks[xr[0]].slot > store.blocks[xr[1]].slot
+            && isChain(xr[1..], store)
+    }
+
+    predicate isChain2(xr: seq<Root>, store: Store)  
+        decreases xr
+    {
+        |xr| >= 1
+        &&
         // (forall i :: 0 <= i < |xr| ==> xr[i] in store.blocks.Keys)
         xr[0] in store.blocks.Keys
         &&  
@@ -119,7 +140,7 @@ module ForkChoiceTypes {
             xr[1] in store.blocks.Keys
             && store.blocks[xr[0]].parent_root == xr[1] 
             && store.blocks[xr[0]].slot > store.blocks[xr[1]].slot
-            && isChain(xr[1..], store)
+            && isChain2(xr[1..], store)
     }
 
     /**
